nearly finish invariant API

IrisCore/Invariant.thy
@@ -1,260 +1,263 @@
 theory Invariant
-imports DerivedConstructions BaseLogicShallow Frac AuthHeap Misc "../SpanningTree/SpanningTreeCameras"
-  Namespace iPropShallow
+imports ViewShift
 begin
 
-subsection \<open> Invariants \<close>
+subsubsection \<open>Impredicative Invariants\<close>
 
-text \<open>The modular invariant camera based on the heap camera\<close>
-definition own_inv :: "inv \<Rightarrow> iprop" ("Own\<^sub>i _") where
-  "own_inv i = Own(constr_inv i)"
+text \<open>Semantic invariant definition\<close>
+definition inv :: "namespace \<Rightarrow> iprop \<Rightarrow> iprop" where
+  "inv N P = \<box>(\<forall>\<^sub>u E. ((\<upharpoonleft>((dnames N) \<subseteq>\<^sub>d E)) \<longrightarrow>\<^sub>u 
+    (\<Turnstile>{E,E-(dnames N)}=> ((\<triangleright>P) \<^emph> ((\<triangleright>P) ={E-(dnames N), E}=\<^emph> \<upharpoonleft>True)))))"
 
-context assumes "SORT_CONSTRAINT('c::ucamera)" and "SORT_CONSTRAINT('v::ofe)"
-begin
-
-text \<open>Allocate new invariant map\<close>
-definition ownI :: "name \<Rightarrow> iprop \<Rightarrow> iprop" where
-  "ownI \<iota> P = Own\<^sub>i (map_view_frag \<iota> DfracDiscarded (Next (pre P)),\<epsilon>,\<epsilon>)"
-
-definition inv :: "namespace \<Rightarrow> iprop \<Rightarrow>  iprop" where
-  "inv N P \<equiv> \<exists>\<^sub>u \<iota>. ((\<upharpoonleft>(\<iota>\<in>\<^sub>d dnames N)) \<and>\<^sub>u ownI \<iota> P)"
-
-text \<open>Allocate new enabled invariant map\<close>
-definition ownE :: "name dset \<Rightarrow> iprop" where
-  "ownE E = Own\<^sub>i (\<epsilon>,E,\<epsilon>)"
-
-text \<open>Allocate new disabled invariant map\<close>
-definition ownD :: "name dfset \<Rightarrow> iprop" where
-  "ownD D = Own\<^sub>i (\<epsilon>,\<epsilon>,D)"  
-  
-definition lift_inv_fmap :: "(name,iprop) fmap \<Rightarrow> (name,pre_iprop later) fmap" where
-  "lift_inv_fmap m = Abs_fmap (map_option (Next \<circ> pre) \<circ> (fmlookup m))"
-
-lemma lift_inf_fmap_finite: "(map_option (Next \<circ> pre) \<circ> (fmlookup m)) \<in> {m. finite (dom m)}"
-  by auto
-
-text \<open>World satisfaction, i.e. the invariant that holds all invariants\<close>
-definition wsat :: iprop where
-  "wsat \<equiv> \<exists>\<^sub>u (I::(name,iprop) fmap).
-    ((Own\<^sub>i(map_view_auth (DfracOwn 1) (lift_inv_fmap I),\<epsilon>,\<epsilon>))
-    \<^emph> (sep_map_fmdom (\<lambda>\<iota>. (\<triangleright>(the (fmlookup I \<iota>))) \<^emph> ownD (DFSet {|\<iota>|}) \<or>\<^sub>u (ownE (DSet {\<iota>}))) I)
-  )"
-end
-
-lemma pcore_id_inv: "pcore_id_pred (constr_inv (map_view_frag \<iota> DfracDiscarded (Next (pre P)), \<epsilon>, \<epsilon>))"
-  unfolding constr_inv_def prod_pcore_id_pred
-  by (simp add: \<epsilon>_pcore_id_def) (rule pcore_id_frag[OF discarded_core_id])
-
-lemma persistent_ownI [pers_rule]: "persistent (ownI \<iota> P)"
-  unfolding ownI_def own_inv_def by (rule persistent_core_own2[OF pcore_id_inv])
-
-lemma persistent_inv [pers_rule]: "persistent (inv N P)"
-  unfolding inv_def
-  apply (rule persistent_exists)
-  apply (rule persistent_conj)
-  apply (rule persistent_pure)
-  by (rule persistent_ownI)
-
-lemma constr_inv_valid: "\<lbrakk>valid mv; valid e; valid d\<rbrakk> \<Longrightarrow> valid (constr_inv (mv,e,d))"
-  unfolding constr_inv_def by (auto simp: prod_valid_def \<epsilon>_valid)
-
-lemma ownE_singleton_twice: "ownE (DSet {i}) \<^emph> ownE (DSet {i}) \<turnstile> \<upharpoonleft>False"
-  unfolding ownE_def own_inv_def constr_inv_def
-  apply (rule upred_entails_trans[OF upred_entail_eqR[OF own_op]])
-  apply (rule upred_entails_trans[OF own_valid])
-  apply (simp add: op_prod_def \<epsilon>_left_id op_dset_def)
-  apply transfer
-  by (simp add: prod_n_valid_def \<epsilon>_n_valid valid_raw_dset_def)
-
-lemma ownD_singleton_twice: "ownD (DFSet {|i|}) \<^emph> ownD (DFSet {|i|}) \<turnstile> \<upharpoonleft>False"
-  unfolding ownD_def own_inv_def constr_inv_def
-  apply (auto simp: op_prod_def \<epsilon>_left_id op_dfset_def
-    intro!: upred_entails_trans[OF upred_entail_eqR[OF own_op]] upred_entails_trans[OF own_valid])
-  apply transfer
-  by (simp add: prod_n_valid_def \<epsilon>_n_valid valid_raw_dfset_def)
-  
-lemma ownE_op: "(\<exists>E1' E2'. dset_raw E1 = Some E1' \<and> dset_raw E2 = Some E2' \<and> E1' \<inter> E2' = {})
-  \<Longrightarrow> ownE (E1 \<cdot> E2) \<stileturn>\<turnstile> ownE E1 \<^emph> ownE E2"
-proof -
-  assume "\<exists>E1' E2'. dset_raw E1 = Some E1' \<and> dset_raw E2 = Some E2' \<and> E1' \<inter> E2' = {}"
-  then obtain E1' E2' where assms: "dset_raw E1 = Some E1'" "dset_raw E2 = Some E2'" "E1' \<inter> E2' = {}"
-    by auto
-  then have "E1 = DSet E1'" "E2 = DSet E2'" by (metis dset_raw.elims option.discI option.inject)+
-  with assms(3) have un_op:"DSet (E1' \<union> E2') = E1 \<cdot> E2" unfolding op_dset_def by simp
-  from own_op[of "constr_inv (\<epsilon>,E1,\<epsilon>)" "constr_inv (\<epsilon>,E2,\<epsilon>)"] 
-  have "ownE (E1 \<cdot> E2) \<stileturn>\<turnstile> ownE E1 \<^emph> ownE E2"
-    by (simp add: ownE_def own_inv_def constr_inv_def op_prod_def \<epsilon>_left_id)
-  with un_op show ?thesis by simp
-qed
-
-lemma ownE_op_minus: "E1 \<subseteq>\<^sub>d E2 \<Longrightarrow> ownE (E1 \<cdot> (E2-E1)) \<stileturn>\<turnstile> ownE E1 \<^emph> ownE (E2-E1)"
-proof -
-  assume "E1 \<subseteq>\<^sub>d E2"
-  then have "\<exists>E1' E2'. dset_raw E1 = Some E1' \<and> dset_raw (E2-E1) = Some E2' \<and> E1' \<inter> E2' = {}"
-    using dsubs_dset dsubs_minus_inter by fastforce
-  from ownE_op[OF this] show ?thesis .
-qed
-  
-lemma auth_map_both_validI: 
-  "\<V>(constr_inv (map_view_auth (DfracOwn 1) m,\<epsilon>,\<epsilon>) \<cdot> constr_inv (map_view_frag k dq v,\<epsilon>,\<epsilon>)) \<turnstile>
-    (fmlookup m k =\<^sub>u Some v) \<and>\<^sub>u \<upharpoonleft>(valid dq)"
-unfolding constr_inv_def op_prod_def
-apply (simp add: \<epsilon>_left_id auth_comb_opL split: prod.splits)
-apply transfer'
-apply (simp add: prod_n_valid_def \<epsilon>_n_valid valid_raw_option_def \<epsilon>_option_def)
-using map_view_both_valid by fastforce
-
-lemma invariant_lookup: 
-  "Own\<^sub>i (map_view_auth (DfracOwn 1) (lift_inv_fmap I),\<epsilon>,\<epsilon>) \<^emph> ownI \<iota> P \<turnstile> 
-  (\<exists>\<^sub>u Q. \<upharpoonleft>(fmlookup I \<iota> = Some Q) \<^emph> \<triangleright>(Q=\<^sub>uP))"
-  unfolding ownI_def own_inv_def
-  apply (rule upred_entails_trans[OF upred_entail_eqR[OF own_op]])
-  apply (rule upred_entails_trans[OF own_valid])
-  apply (rule upred_entails_trans[OF auth_map_both_validI])
-  apply transfer'
-  apply (auto simp: lift_inv_fmap_def valid_raw_dfrac_def valid_def n_equiv_option_def 
-    n_equiv_later_def Abs_fmap_inverse[OF lift_inf_fmap_finite])
-  apply (metis dual_order.refl n_incl_def ofe_refl prod_cases3 total_n_inclI)
-  by (metis \<epsilon>_left_id ofe_refl prod_cases3) 
-
-lemma lookup_pers [pers_rule]: "persistent (\<exists>\<^sub>u Q. \<upharpoonleft>(fmlookup I \<iota> = Some Q) \<^emph> \<triangleright>(Q=\<^sub>uP))"
-  by pers_solver
-
-lemma ownI_open: "wsat \<^emph> ownI i P \<^emph> ownE (DSet {i}) \<turnstile> wsat \<^emph> (\<triangleright>P) \<^emph> ownD (DFSet {|i|})"
-unfolding wsat_def
-apply (rule pull_exists_antecedent2)
-apply (rule upred_existsE')
-apply (rule upred_entails_trans[OF upred_entails_eq[OF upred_sep_comm]])
-apply (rule upred_entails_trans[OF upred_sep_assoc])
-apply (rule upred_entails_trans[OF upred_sep_assoc'])
-apply (rule upred_entails_trans[OF upred_sep_comm3M])
-apply (rule upred_entails_trans[OF upred_sep_assoc_rev])
-apply (rule upred_entails_exchange[OF  persistent_keep[OF lookup_pers invariant_lookup]])
-apply (rule upred_entails_trans[OF upred_sep_assoc])
-apply (rule pull_exists_antecedentR)
-apply (rule upred_existsE')
-apply (rule upred_entails_trans[OF upred_sep_assoc])
-apply (rule upred_entails_trans[OF upred_entails_eq[OF upred_sep_comm]])
-apply (rule upred_entails_trans[OF upred_sep_assoc])
-apply (rule upred_pure_impl)
-apply (rule upred_entails_trans[OF upred_sep_assoc])
-apply (rule upred_entails_trans[OF upred_entails_eq[OF upred_sep_comm]])
-apply (rule upred_entails_trans[OF upred_sep_assoc])+
-apply (simp add: sep_map_dom_delete)
-apply (rule upred_entails_trans[OF upred_sep_assoc])
+lemma inv_raw_acc: "dnames N \<subseteq>\<^sub>d E \<Longrightarrow> 
+  ((inv_raw N P) ={E, E-(dnames N)}=\<^emph> ((\<triangleright>P) \<^emph> ((\<triangleright>P) ={E-(dnames N), E}=\<^emph> \<upharpoonleft>True)))"
+apply (auto simp: fancy_upd_def upred_sep_assoc_eq inv_raw_def intro!: upred_wand_holdsI upred_existsE')
+apply (rule upred_entails_trans[OF upred_entail_eqR[OF persistent_holds_sep']], pers_solver)
+apply (auto intro!: upred_entails_trans[OF upred_entails_eq[OF upred_sep_comm]] upred_pure_impl)
+apply (auto simp: upred_sep_assoc_eq intro!: upred_wandI)
+apply (subst dsubs_op_minus[of "dnames N"], assumption)
+apply (auto simp: upred_sep_assoc_eq intro!: upred_entails_substE[OF upred_entail_eqL[OF ownE_op_minus]])
+subgoal for i
+unfolding delem_dsubs[of i "dnames N"]
+apply (subst dsubs_op_minus[of "DSet {i}" "dnames N"], assumption)
 apply (rule upred_entails_trans[OF upred_sep_comm2R])
-apply (rule upred_disjE')
-subgoal for I Q
-  apply (rule upred_entails_trans[OF upred_sep_assoc])
-  apply (rule upred_frame)
-  apply (rule upred_entails_trans[OF upred_sep_comm4_2])
-  apply (rule upred_entails_trans[OF upred_sep_comm3M])
-  apply (rule persistent_split[OF persistent_later[OF persistent_eq]])
-  subgoal
-    apply (rule upred_entails_trans[OF upred_entail_eqR[OF upred_later_sep]])
-    apply (rule upred_later_mono)
-    apply (rule upred_entails_trans[OF upred_entails_eq[OF upred_sep_comm]])
-    apply (simp add: upred_eq_comm)
-    apply (rule upred_eqE)
-  by simp
-  apply(rule upred_existsI[of _ _ "I"])
-  apply (rule upred_entails_trans[OF upred_entails_eq[OF upred_sep_comm]])
-  apply (rule upred_entails_trans[OF upred_sep_assoc])
-  apply (rule upred_entails_trans[OF upred_entails_eq[OF upred_sep_comm]])
-  apply (rule upred_entails_trans[OF upred_sep_assoc])+
-  apply (rule upred_entails_trans[OF upred_entails_eq[OF upred_sep_comm]])
-  apply (rule upred_entails_trans[OF upred_sep_assoc])+
-  apply (rule upred_entails_trans[OF upred_entails_eq[OF upred_sep_comm]])
-  apply (rule upred_entails_trans[OF upred_sep_assoc])
-  apply (rule upred_entails_trans[OF _ upred_entails_eq[OF upred_sep_comm]])
-  apply (rule upred_frame)
-  apply (simp add: sep_map_dom_delete)
-  apply (rule upred_entails_trans[OF upred_sep_assoc])+
-  apply (rule upred_entails_trans[OF upred_sep_comm2R])
-  apply (rule upred_frame)
-  apply (rule upred_disjIR)
-  apply (rule upred_entails_trans[OF upred_sep_comm2R])
-by (rule upred_weakeningR)
-apply (rule upred_entails_trans[OF upred_entails_eq[OF upred_sep_comm2L]])
-apply (rule upred_entails_trans[OF upred_sep_assoc'])
-apply (rule upred_entails_trans[OF upred_sep_assoc_rev])
-apply (rule upred_entails_exchange[OF ownE_singleton_twice])
-by simp
-
-lemma ownI_close: "wsat \<^emph> ownI i P \<^emph> (\<triangleright> P) \<^emph> ownD (DFSet {|i|}) \<turnstile> wsat \<^emph> ownE (DSet {i})"
-apply (simp add: wsat_def)
-apply (auto simp: pull_exists_eq intro!: upred_existsE')
-apply (rule upred_entails_trans[OF upred_sep_comm3M])
-apply (rule upred_entails_trans[OF upred_sep_comm2R])
-apply (rule upred_entails_trans[OF upred_entails_eq[OF upred_sep_comm2L]])
-apply (auto simp: upred_sep_assoc_eq)
+apply (auto simp: upred_sep_assoc_eq intro!: upred_entails_substE[OF 
+    upred_entail_eqL[OF ownE_op_minus], of "DSet {i}" "dnames N"] upred_entails_trans[OF _ updI]
+    upred_entails_trans[OF _ except_zeroI])
 apply (rule upred_entails_trans[OF upred_sep_comm4_2])
-apply (rule upred_entails_trans[OF upred_entails_eq[OF upred_sep_comm2L]])
-apply (auto simp: upred_sep_assoc_eq)
-apply (rule upred_entails_exchange[OF persistent_keep[OF lookup_pers invariant_lookup], unfolded upred_sep_assoc_eq])
-subgoal for I 
-apply (auto simp: upred_sep_assoc_eq intro!: upred_existsI[of _ _ I] pull_exists_antecedentR upred_existsE')
 apply (rule upred_entails_trans[OF upred_sep_comm2R])
-apply (auto simp: sep_map_dom_delete upred_sep_assoc_eq intro!: upred_pure_impl)
-apply (rule upred_entails_trans[OF upred_entails_eq[OF upred_sep_comm]])
+apply (rule upred_entails_trans[OF upred_sep_comm3M])
+apply (rule upred_entails_trans[OF upred_sep_comm4_1])
+apply (rule upred_entails_trans[OF upred_sep_comm4_2])
+apply (rule upred_entails_trans[OF upred_sep_comm3M])
+apply (rule upred_entails_trans[OF upred_sep_comm2R])
+apply (rule upred_entails_substE[OF upred_entail_eqR[OF persistent_dupl]])
+apply pers_solver
 apply (simp add: upred_sep_assoc_eq)
-apply (rule upred_entails_trans[OF upred_sep_comm4_2])
 apply (rule upred_entails_trans[OF upred_sep_comm3M])
-apply (rule upred_entails_trans[OF upred_sep_comm2R])
-apply (auto simp: upred_sep_assoc_eq intro!: upred_disjE')
-subgoal for Q  
-  apply (rule upred_entails_trans[OF upred_sep_comm6_2R])
-  by (auto intro!: upred_entails_exchange[OF ownD_singleton_twice, unfolded upred_sep_assoc_eq])
-apply (auto simp: upred_sep_assoc_eq intro!: upred_frame)
-apply (rule upred_entails_trans[OF upred_entails_eq[OF upred_sep_comm2L]])
-apply (rule upred_entails_trans[OF upred_sep_comm2R])
-apply (auto simp: upred_sep_assoc_eq intro!: upred_frame)
-apply (rule upred_entails_trans[OF upred_entails_eq[OF upred_sep_comm2L]])
+apply (rule upred_entails_trans[OF upred_sep_comm3L])
 apply (simp add: upred_sep_assoc_eq)
-apply (rule upred_entails_trans[OF upred_sep_comm4_2])
+apply (rule upred_entails_trans[OF upred_sep_comm2R])
+apply (rule upred_entails_substE[OF ownI_open, unfolded upred_sep_assoc_eq])
+apply (rule upred_entails_trans[OF _ upred_sep_comm2R])
+apply (rule upred_entails_trans[OF upred_sep_comm2R])
+apply (rule upred_frame)
+apply (rule upred_entails_trans[OF _ upred_sep_comm2R])
+apply (rule upred_entails_trans[OF upred_sep_comm3L])
+apply (simp add: upred_sep_assoc_eq)
 apply (rule upred_entails_trans[OF upred_sep_comm3M])
 apply (rule upred_entails_trans[OF upred_sep_comm2R])
+apply (rule upred_frame)
 apply (rule upred_entails_trans[OF _ upred_entails_eq[OF upred_sep_comm]])
-apply (auto simp: upred_sep_assoc_eq intro!: upred_frame upred_disjIL)
+apply (rule upred_entails_trans[OF upred_sep_comm2R])
+apply (auto simp: upred_sep_assoc_eq intro!: upred_frame upred_wandI)
+apply (rule upred_entails_trans[OF upred_entails_eq[OF upred_sep_comm]])
+apply (simp add: upred_sep_assoc_eq)
+apply (rule upred_entails_trans[OF upred_sep_comm2R])
+apply (rule upred_entails_trans[OF upred_sep_comm3M])
+apply (rule upred_entails_trans[OF upred_sep_comm2R])
+apply (rule upred_entails_trans[OF upred_sep_comm4_2])
+apply (rule upred_entails_substE[OF ownI_close, unfolded upred_sep_assoc_eq])
+apply (rule upred_entails_trans[OF upred_sep_comm3M])
+apply (rule upred_entails_trans[OF upred_sep_comm2R])
+apply (auto simp: dsubs_op_minus[symmetric] intro!: upred_entails_substE[OF 
+    upred_entail_eqR[OF ownE_op_minus], unfolded upred_sep_assoc_eq])
 apply (rule upred_entails_trans[OF upred_entails_eq[OF upred_sep_comm2L]])
-by (auto intro!: upred_entails_trans[OF upred_weakeningR2] 
-  upred_entails_trans[OF upred_entail_eqR[OF upred_later_sep]] upred_later_mono upred_eqE)
+apply (rule upred_entails_trans[OF upred_sep_comm2R])
+apply (auto simp: dsubs_op_minus[symmetric] intro!: upred_entails_substE[OF 
+    upred_entail_eqR[OF ownE_op_minus], unfolded upred_sep_assoc_eq] upred_entails_trans[OF _ updI]
+    upred_entails_trans[OF _ except_zeroI])
+apply (rule upred_entails_trans[OF _ upred_sep_comm2R])
+by (auto simp: upred_true_sep intro!: upred_frame)
 done
 
-lemma ownI_alloc: "(\<forall>E::name dfset. \<exists>i. \<not>i\<in>\<^sub>fE \<and> \<phi> i) \<Longrightarrow> 
-  (wsat \<^emph> \<triangleright> P) ==\<^emph> (\<exists>\<^sub>u i. \<upharpoonleft>(\<phi> i) \<^emph> wsat \<^emph> ownI i P)"
-apply (auto simp: wsat_def pull_exists_eq intro!: upred_wand_holdsI upred_existsE')
-apply (rule add_holds[OF own_unit,unfolded bupd_emp[OF upred_own_nothing_emp_eq]])
-apply (rule upred_entails_exchange[OF upred_wand_holdsE[OF own_updateP]])
-sorry (* Axiomatized as this requires too much low level ghost state reasoning for which I'd need to add
-    way more lemmata and things. *)
+lemma fresh_inv_name: "\<exists>\<iota>. \<not> (\<iota> \<in>\<^sub>f E) \<and> \<iota> \<in>\<^sub>d dnames N"
+proof -
+  from infinite_names dset_of_finite_finite have "dnames N - dset_of_finite E \<noteq> DSet {}"
+    unfolding dnames_def apply (cases E) apply auto using finite_fset infinite_super apply blast 
+    using not_no_names by simp
+  then obtain \<iota> where "\<iota> \<in>\<^sub>d dnames N - dset_of_finite E" unfolding dnames_def by (cases E) auto
+  then have "\<not> (\<iota> \<in>\<^sub>f E) \<and> \<iota> \<in>\<^sub>d dnames N" apply (cases E) by (auto simp add: dnames_def fmember.rep_eq)
+  then show ?thesis by blast
+qed
 
-lemma ownI_alloc_open: "(\<forall>E::name dfset. \<exists>i. \<not>i\<in>\<^sub>fE \<and> \<phi> i) \<Longrightarrow> 
-  wsat ==\<^emph> (\<exists>\<^sub>u i. \<upharpoonleft>(\<phi> i) \<^emph> (ownE (DSet {i}) -\<^emph> wsat) \<^emph> ownI i P \<^emph> ownD (DFSet {|i|}))"
-apply (auto simp: wsat_def pull_exists_eq intro!: upred_wand_holdsI upred_existsE')
-sorry (* Axiomatized as this requires too much low level ghost state reasoning for which I'd need to add
-    way more lemmata and things. *)
+lemma inv_raw_alloc: "(\<triangleright>P) ={E}=\<^emph> (inv_raw N P)"
+apply (auto simp: fancy_upd_def upred_sep_assoc_eq intro!: upred_wand_holdsI upred_wandI)
+apply (subst upred_sep_comm2_eq[of wsat])
+apply (rule upred_entails_trans[OF _ upd_mono,OF _ except_zero_sepR])
+apply (auto intro!: upred_entails_trans[OF _ upd_frameL] upred_frame)
+apply (rule upred_wand_holdsE)
+apply (subst upred_sep_comm)
+apply (rule upred_entails_wand_holdsR[OF _ ownI_alloc[of "\<lambda>i. i \<in>\<^sub>d dnames N"], 
+    OF _ allI[OF fresh_inv_name, of id, simplified]])
+apply (rule upd_mono)
+apply (auto intro!: upred_existsE')
+apply (subst upred_sep_comm[of wsat])
+apply (subst upred_sep_comm2_eq)
+apply (auto intro!: upred_entails_trans[OF _ except_zeroI] upred_frame)
+unfolding inv_raw_def
+subgoal for i
+apply (rule upred_existsI[of _ _ i])
+apply (subst upred_sep_comm)
+by (auto simp: dnames_def intro!:upred_pure_impl upred_entails_conjI upred_pureI)
+done
 
-lemma wsat_alloc: "\<Rrightarrow>\<^sub>b (\<exists>\<^sub>u _::inv. wsat \<^emph> ownE (DSet UNIV))"
-apply (auto simp: upred_holds_entails)
-apply (rule add_own[of "constr_inv (map_view_auth (DfracOwn 1) fmempty,\<epsilon>,\<epsilon>)", 
-  OF constr_inv_valid[OF map_view_auth_valid \<epsilon>_valid \<epsilon>_valid]])
-apply (rule add_own[of "constr_inv (\<epsilon>,DSet UNIV,\<epsilon>)", 
-  OF constr_inv_valid[OF \<epsilon>_valid _ \<epsilon>_valid]])
-apply (simp add: valid_raw_dset_def valid_def)
-apply (rule add_own[of "constr_inv (\<epsilon>,\<epsilon>,DFSet {||})", 
-  OF constr_inv_valid[OF \<epsilon>_valid \<epsilon>_valid _], unfolded \<epsilon>_dfset_def[symmetric], OF \<epsilon>_valid])
-apply (auto simp: wsat_def pull_exists_eq own_inv_def ownE_def ownD_def 
-  intro!: upred_entails_trans[OF _ updI])
-apply (rule upred_existsI)
-apply (rule upred_existsI[of _ _ fmempty])
+lemma inv_raw_alloc_open: "dnames N \<subseteq>\<^sub>d E \<Longrightarrow>
+  \<Turnstile>{E, E-dnames N}=> (inv_raw N P \<^emph> ((\<triangleright>P) ={E-dnames N, E}=\<^emph> upred_emp))"
+unfolding fancy_upd_def
+apply (rule upred_wand_holdsI)
+apply (rule upred_wandE)
+apply (rule upred_entails_trans[OF upred_wand_holdsE[OF ownI_alloc_open[of "\<lambda>i. i \<in>\<^sub>d dnames N"]],
+  OF allI[OF fresh_inv_name, of id, simplified], of P])
+apply (auto simp: pull_exists_eq intro!: upred_wandI upred_entails_trans[OF upd_frameL] upd_mono upred_existsE')
+apply (rule upred_entails_trans[OF upred_sep_comm4_1])
+apply (rule upred_entails_trans[OF upred_sep_comm4_2])
+apply (rule upred_entails_trans[OF upred_sep_comm3M])
 apply (rule upred_entails_trans[OF upred_sep_comm2R])
-apply (auto intro!: upred_frame)
-apply (auto simp: lift_inv_fmap_def fmempty.rep_eq fmempty_def[symmetric] sep_fold_fset_def 
-  comp_fun_commute.ffold_empty[OF sep_P_comp_fun_commute]  intro!: upred_frame)
+apply (rule upred_pure_impl)
+apply (rule upred_entails_trans[OF upred_sep_comm3M])
+apply (rule upred_entails_trans[OF upred_sep_comm2R])
+subgoal for i
+apply (rule split_trans[of _ "ownE E \<^emph> ownI i P" "(ownE (DSet {i}) -\<^emph> wsat) \<^emph> ownD (DFSet {|i|}) \<^emph> ownI i P" 
+  "ownE (DSet {i}) \<^emph> ownE (dnames N - DSet {i}) \<^emph> ownE (E - dnames N)", unfolded upred_sep_assoc_eq])
+apply(rule can_be_split_R_R[OF persistent_dupl_split[OF persistent_ownI], unfolded upred_sep_assoc_eq])
+apply (rule upred_entails_trans[OF _ upred_sep_comm2R])
+apply (rule upred_entails_trans[OF _ upred_entails_eq[OF upred_sep_comm2L]])
+apply (auto simp: delem_dsubs dsubs_op_minus[symmetric] intro!: upred_entails_substI[OF 
+    upred_entail_eqL[OF ownE_op_minus], unfolded upred_sep_assoc_eq])
+apply (rule upred_entails_trans[OF _ upred_entails_eq[OF upred_sep_comm]])
+apply (auto simp: delem_dsubs dsubs_op_minus[symmetric] upred_weakeningL upred_sep_assoc_eq
+  intro!: upred_entails_trans[OF _ upred_entail_eqL[OF ownE_op_minus], unfolded upred_sep_assoc_eq] 
+  upred_entails_trans[OF _ except_zeroI])
+apply (rule upred_entails_trans[OF upred_sep_comm4_2])
+apply (rule upred_entails_trans[OF upred_sep_comm3M])
+apply (rule upred_entails_trans[OF upred_sep_comm2R])
+apply (rule upred_entails_trans[OF _ upred_sep_comm3M])
+apply (rule upred_entails_trans[OF _ upred_sep_comm2R])
+apply (rule upred_frame)
+apply (rule upred_entails_trans[OF upred_sep_comm3M])
+apply (rule upred_entails_trans[OF upred_sep_comm4_1])
+apply (rule upred_entails_trans[OF upred_sep_comm4_2])
+apply (rule split_frame[of _ "ownE (DSet {i}) \<^emph> (ownE (DSet {i}) -\<^emph> wsat) \<^emph> ownI i P" 
+  "ownE (dnames N - DSet {i}) \<^emph> ownD (DFSet {|i|})\<^emph> ownI i P" _ wsat
+  "inv_raw N P \<^emph> ((\<triangleright>P) -\<^emph> (wsat \<^emph> ownE (E - dnames N)) ==\<^emph> \<diamondop>(wsat \<^emph> ownE E \<^emph> upred_emp))", 
+  unfolded upred_sep_assoc_eq])
+apply (rule can_be_split_mono[OF _ persistent_dupl_split[OF persistent_ownI], unfolded upred_sep_assoc_eq])
+apply (rule can_be_split_rev)
+apply (rule can_be_split_refl)
+subgoal unfolding can_be_split_def by (simp add: upred_entails_eq_eq upred_sep_assoc_eq)
+apply (auto intro: upred_entails_trans[OF upred_weakeningL] upred_wand_apply)
+apply (rule split_frame[of _ "ownI i P" _ _ "inv_raw N P"])
+apply (rule can_be_split_rev)
+apply (rule persistent_dupl_split, pers_solver)
+apply (rule can_be_split_refl)
+apply (auto simp: inv_raw_def delem_dsubs upred_true_conj' upred_sep_assoc_eq intro!: upred_existsI[of _ _ i] upred_wandI)
+apply (rule upred_entails_trans[OF upred_entails_eq[OF upred_sep_comm]]; simp add: upred_sep_assoc_eq)
+apply (rule upred_entails_trans[OF upred_sep_comm4_2])
+apply (rule upred_entails_trans[OF upred_sep_comm3M])
+apply (rule upred_entails_trans[OF upred_sep_comm2R])
+apply (rule upred_entails_trans[OF upred_sep_comm3M])
+apply (rule upred_entails_trans[OF upred_sep_comm4_2])
+apply (rule upred_entails_substE[OF ownI_close, unfolded upred_sep_assoc_eq])
+apply (rule upred_entails_trans[OF upred_sep_comm3M])
+apply (rule upred_entails_trans[OF upred_sep_comm2R])
+apply (auto simp: dsubs_op_minus[symmetric] intro!: upred_entails_substE[OF 
+    upred_entail_eqR[OF ownE_op_minus], unfolded upred_sep_assoc_eq])
 apply (rule upred_entails_trans[OF upred_entails_eq[OF upred_sep_comm2L]])
 apply (rule upred_entails_trans[OF upred_sep_comm2R])
-by (auto simp: upred_weakeningL intro!: upred_frame)
+by (auto simp: dsubs_op_minus[symmetric] upred_true_sep intro!: upred_entails_substE[OF 
+    upred_entail_eqR[OF ownE_op_minus], unfolded upred_sep_assoc_eq] upred_entails_trans[OF _ updI]
+    upred_entails_trans[OF _ except_zeroI])
+done
+
+lemma inv_raw_to_inv: "inv_raw N P -\<^emph> inv N P"
+unfolding inv_def
+apply (auto intro!: upred_wand_holdsI upred_entails_trans[OF _ upred_entail_eqL[OF pers_forall]] 
+  upred_forallI upred_entails_trans[OF _ upred_entail_eqR[OF upred_pers_impl_pure]] upred_implI_pure)
+subgoal for E
+apply (rule add_holds[OF inv_raw_acc[of N E P]], assumption)
+apply (auto intro!: upred_entails_trans[OF upred_wand_apply])
+apply (auto intro!: upred_entails_trans[OF fupd_mono[OF upred_wand_apply]] 
+  upred_entails_trans[OF upred_holds_entails'[OF fupd_mask_subseteq[of "E-dnames N" E]]])
+using dsubs_dset apply fastforce
+using upred_pers_mono[OF fupd_mono[OF upred_wand_apply]]
+sorry
+done
+
+text \<open>
+  The follow lemmata are the public API for invariants and should be enough to handle most proofs
+  with invariants.
+\<close>
+
+lemma persistent_inv [pers_rule]: "persistent (inv N P)"
+  unfolding inv_def by pers_solver
+
+lemma inv_alter: "inv N P -\<^emph> (\<triangleright>\<box>(P -\<^emph> (Q \<^emph> (Q-\<^emph>P)))) -\<^emph> inv N Q"
+apply (auto simp: inv_def intro!: upred_wand_holds2I upred_entails_trans[OF _ upred_entail_eqL[OF 
+    pers_forall]] upred_forallI upred_entails_trans[OF _ upred_entail_eqR[OF upred_pers_impl_pure]]
+    upred_implI_pure)
+apply (rule persistent_persisI, pers_solver)
+apply (rule upred_entails_trans[OF upred_entails_eq[OF upred_sep_comm]])
+subgoal for E
+apply (auto intro!: upred_entails_substE[OF upred_persis_mono[OF upred_forall_inst[of _ E]]] 
+  upred_entails_substE[OF upred_persis_mono[OF upred_entail_eqL[OF upred_emp_impl]]])
+apply (auto simp: upred_sep_assoc_eq intro!: upred_entails_substE[OF upred_persisE] fupd_frame_mono)
+apply (rule upred_entails_trans[OF upred_sep_comm2R])
+apply (rule upred_entails_trans[OF upred_entails_eq[OF upred_sep_comm2L]])
+apply (rule upred_entails_trans[OF upred_sep_comm2R])
+apply (rule split_trans[OF _ upred_entails_trans[OF upred_entail_eqR[OF upred_later_sep] upred_later_mono[OF
+  upred_persis_mono_frame[OF upred_wand_apply[of P "Q\<^emph>(Q-\<^emph>P)"]]]]])
+apply (rule can_be_split_sepL)
+apply (rule can_be_split_rev)
+apply (rule can_be_split_refl)
+apply (auto intro!: split_frame[OF _ can_be_split_refl, of _ "\<triangleright>Q"])
+apply (rule can_be_split_sepR)
+unfolding can_be_split_def
+apply (rule upred_later_sep)
+apply (rule upred_wandI)
+apply (rule upred_entails_trans[OF upred_entails_eq[OF upred_sep_comm2L]])
+apply (rule upred_entails_trans[OF upred_sep_comm2R])
+apply (rule upred_entails_substE[OF upred_entail_eqR[OF upred_later_sep], OF upred_entails_substE[OF
+    upred_later_mono[OF upred_wand_apply]], unfolded upred_sep_assoc_eq])
+apply (rule upred_entails_trans[OF upred_entails_eq[OF upred_sep_comm]])
+by (auto intro: upred_entails_trans[OF upred_wand_apply])
+done
+
+lemma inv_iff: "inv N P -\<^emph> (\<triangleright>\<box>((P \<longrightarrow>\<^sub>u Q) \<and>\<^sub>u (Q\<longrightarrow>\<^sub>uP))) -\<^emph> inv N Q"
+apply (auto intro!: upred_wand_holds2I upred_entails_trans[OF _ upred_wand_holds2E[OF inv_alter], of _ N P])
+apply (auto intro!: upred_sep_mono upred_later_mono)
+apply (rule upred_entails_trans[OF upred_entail_eqR[OF persistent_dupl]], pers_solver)
+apply (rule upred_persis_frame, pers_solver)
+apply (auto intro!: upred_wandI)
+apply (rule split_frame[of _ "((P \<longrightarrow>\<^sub>u Q) \<and>\<^sub>u (Q \<longrightarrow>\<^sub>u P)) \<^emph> P" _ _ Q])
+apply (rule can_be_split_sepL; rule can_be_split_rev; rule can_be_split_refl)
+apply (rule can_be_split_refl)
+apply (rule upred_entails_trans[OF upred_entails_conj_sep])
+apply (subst upred_conj_comm)
+apply (subst upred_conj_comm2R)
+apply (auto simp: upred_weakeningR' intro: upred_entails_substE'[OF upred_impl_apply, unfolded upred_conj_assoc])
+apply (rule upred_entails_trans[OF upred_persisE])
+apply (rule upred_wandI)
+apply (rule upred_entails_trans[OF upred_entails_conj_sep])
+apply (subst upred_conj_comm2R)
+by (auto simp: upred_weakeningR' intro: upred_entails_substE'[OF upred_impl_apply, unfolded upred_conj_assoc])
+
+lemma inv_alloc: "(\<triangleright>P) ={E}=\<^emph> inv N P"
+  by (auto intro!: upred_wand_holdsI upred_entails_trans[OF _ fupd_mono[OF upred_wand_holdsE[OF 
+    inv_raw_to_inv]]] upred_wand_holdsE[OF inv_raw_alloc])
+
+lemma inv_alloc_open: "dnames N \<subseteq>\<^sub>d E \<Longrightarrow>
+  \<Turnstile>{E, E-dnames N}=> (inv N P \<^emph> ((\<triangleright>P) ={E-dnames N, E}=\<^emph> upred_emp))"
+apply (auto simp: upred_holds_entails)
+apply (rule add_holds[OF inv_raw_alloc_open[of N E P]], simp)
+apply (rule upred_entails_trans[OF upred_entails_eq[OF upred_sep_comm]])
+apply (rule upred_entails_trans[OF upred_weakeningL])
+by (auto simp: upred_wand_holdsE[OF inv_raw_to_inv] intro!: fupd_mono upred_sep_mono)
+
+lemma inv_acc: "dnames N \<subseteq>\<^sub>d E \<Longrightarrow> 
+  ((inv N P) ={E, E-(dnames N)}=\<^emph> ((\<triangleright>P) \<^emph> ((\<triangleright>P) ={E-(dnames N), E}=\<^emph> \<upharpoonleft>True)))"
+  by (auto simp: inv_def intro!: upred_wand_holdsI upred_entails_trans[OF upred_persisE]
+    upred_entails_trans[OF upred_forall_inst[of _ E]] upred_entails_trans[OF upred_entail_eqL[OF upred_emp_impl]])
 
 subsubsection \<open>Cancelable Invariants\<close>
 type_synonym cinvG = frac
@@ -265,18 +268,16 @@ lemma cinv_persistent: "persistent (cinv N P)"
   unfolding cinv_def by (rule persistent_inv)
 
 lemma timeless_cinv_own: "timeless (cinv_own p)"
-unfolding timeless_def cinv_own_def constr_cinv_def except_zero_def
-apply transfer
-by (simp add: n_incl_incl del: \<epsilon>_dfset_def \<epsilon>_dset_def)
+  unfolding timeless_def cinv_own_def constr_cinv_def except_zero_def
+  by transfer (simp add: n_incl_incl)
 
 lemma cinv_own_valid: "upred_holds (cinv_own q1 -\<^emph> cinv_own q2 -\<^emph> \<upharpoonleft>(q1\<cdot>q2\<le>1))"
 unfolding cinv_own_def
 apply (rule upred_entails_wand_holdsR2[OF _ own_valid2])
-apply (simp add: constr_cinv_def op_prod_def \<epsilon>_left_id op_option_def del: \<epsilon>_dfset_def \<epsilon>_dset_def)
-apply (simp add: upred_entails.rep_eq upred_valid.rep_eq upred_pure.rep_eq prod_n_valid_def \<epsilon>_n_valid 
-  del: \<epsilon>_dfset_def \<epsilon>_dset_def)
+apply (simp add: constr_cinv_def op_prod_def \<epsilon>_left_id op_option_def)
+apply (simp add: upred_entails.rep_eq upred_valid.rep_eq upred_pure.rep_eq prod_n_valid_def \<epsilon>_n_valid)
 apply (simp add: valid_raw_option_def valid_frac[symmetric] split: option.splits)
-by (metis dcamera_valid_iff less_eq_frac.rep_eq one_frac.rep_eq one_frac_def valid_raw_frac.rep_eq)
+by (metis dcamera_valid_iff less_eq_frac.rep_eq one_frac.rep_eq valid_raw_frac.rep_eq)
 
 lemma cinv_own_1_l: "upred_holds (cinv_own 1 -\<^emph> cinv_own q -\<^emph> \<upharpoonleft>False)"
 proof (rule upred_wand_holds2I)
