IrisCore/ViewShift.thy
@@ -1,8 +1,12 @@
 theory ViewShift
-imports Invariant
+imports WorldSatisfaction
 begin
 
 subsubsection \<open>Fancy updates\<close>
+text \<open>
+  Fancy updates describe steps between different sets of opened/closed invariants and are thus
+  the basis for the impredicative invariant API.
+\<close>
 
 type_synonym mask = "name dset"
 
@@ -20,105 +24,61 @@ abbreviation linear_vs :: "iprop \<Rightarrow> mask \<Rightarrow> iprop \<Righta
   "linear_vs P \<E> Q \<equiv> P ={\<E>,\<E>}=> Q"
   
 lemma fupd_mono: "P\<turnstile>Q \<Longrightarrow> \<Turnstile>{\<E>\<^sub>1, \<E>\<^sub>2}=>P \<turnstile> \<Turnstile>{\<E>\<^sub>1, \<E>\<^sub>2}=>Q"
-unfolding fancy_upd_def
-apply (rule upred_wandI)
-unfolding wsat_def ownE_def ownD_def sep_map_set_def except_zero_def
-sorry
-
-text \<open>Semantic invariant definition\<close>
-definition sinv :: "namespace \<Rightarrow> iprop \<Rightarrow> iprop" where
-  "sinv N P = \<box>(\<forall>\<^sub>u E. ((\<upharpoonleft>((dnames N) \<subseteq>\<^sub>d E)) \<longrightarrow>\<^sub>u 
-    ((\<Turnstile>{E,E-(dnames N)}=> (\<triangleright>P)) \<^emph> ((\<triangleright>P) ={E-(dnames N), E}=\<^emph> \<upharpoonleft>True))))"
-
-lemma inv_acc: "dnames N \<subseteq>\<^sub>d E \<Longrightarrow> 
-  ((inv N P) ={E, E-(dnames N)}=\<^emph> ((\<triangleright>P) \<^emph> ((\<triangleright>P) ={E-(dnames N), E}=\<^emph> \<upharpoonleft>True)))"
-apply (auto simp: fancy_upd_def upred_sep_assoc_eq inv_def intro!: upred_wand_holdsI upred_existsE')
-apply (rule upred_entails_trans[OF upred_entail_eqR[OF persistent_holds_sep']], pers_solver)
-apply (auto intro!: upred_entails_trans[OF upred_entails_eq[OF upred_sep_comm]] upred_pure_impl)
-apply (auto simp: upred_sep_assoc_eq intro!: upred_wandI)
-apply (subst dsubs_op_minus[of "dnames N"], assumption)
-apply (auto simp: upred_sep_assoc_eq intro!: upred_entails_exchange[OF upred_entail_eqL[OF ownE_op_minus]])
-subgoal for i
-unfolding delem_dsubs[of i "dnames N"]
-apply (subst dsubs_op_minus[of "DSet {i}" "dnames N"], assumption)
-apply (rule upred_entails_trans[OF upred_sep_comm2R])
-apply (auto simp: upred_sep_assoc_eq intro!: upred_entails_exchange[OF 
-    upred_entail_eqL[OF ownE_op_minus], of "DSet {i}" "dnames N"] upred_entails_trans[OF _ updI]
-    upred_entails_trans[OF _ except_zeroI])
-apply (rule upred_entails_trans[OF upred_sep_comm4_2])
-apply (rule upred_entails_trans[OF upred_sep_comm2R])
-apply (rule upred_entails_trans[OF upred_sep_comm3M])
-apply (rule upred_entails_trans[OF upred_sep_comm4_1])
-apply (rule upred_entails_trans[OF upred_sep_comm4_2])
-apply (rule upred_entails_trans[OF upred_sep_comm3M])
-apply (rule upred_entails_trans[OF upred_sep_comm2R])
-apply (rule upred_entails_exchange[OF upred_entail_eqR[OF persistent_dupl]])
-apply pers_solver
-apply (simp add: upred_sep_assoc_eq)
-apply (rule upred_entails_trans[OF upred_sep_comm3M])
-apply (rule upred_entails_trans[OF upred_sep_comm3L])
-apply (simp add: upred_sep_assoc_eq)
-apply (rule upred_entails_trans[OF upred_sep_comm2R])
-apply (rule upred_entails_exchange[OF ownI_open, unfolded upred_sep_assoc_eq])
-apply (rule upred_entails_trans[OF _ upred_sep_comm2R])
-apply (rule upred_entails_trans[OF upred_sep_comm2R])
-apply (rule upred_frame)
-apply (rule upred_entails_trans[OF _ upred_sep_comm2R])
-apply (rule upred_entails_trans[OF upred_sep_comm3L])
-apply (simp add: upred_sep_assoc_eq)
-apply (rule upred_entails_trans[OF upred_sep_comm3M])
-apply (rule upred_entails_trans[OF upred_sep_comm2R])
-apply (rule upred_frame)
-apply (rule upred_entails_trans[OF _ upred_entails_eq[OF upred_sep_comm]])
-apply (rule upred_entails_trans[OF upred_sep_comm2R])
-apply (auto simp: upred_sep_assoc_eq intro!: upred_frame upred_wandI)
-apply (rule upred_entails_trans[OF upred_entails_eq[OF upred_sep_comm]])
-apply (simp add: upred_sep_assoc_eq)
-apply (rule upred_entails_trans[OF upred_sep_comm2R])
-apply (rule upred_entails_trans[OF upred_sep_comm3M])
-apply (rule upred_entails_trans[OF upred_sep_comm2R])
-apply (rule upred_entails_trans[OF upred_sep_comm4_2])
-apply (rule upred_entails_exchange[OF ownI_close, unfolded upred_sep_assoc_eq])
-apply (rule upred_entails_trans[OF upred_sep_comm3M])
-apply (rule upred_entails_trans[OF upred_sep_comm2R])
-apply (auto simp: dsubs_op_minus[symmetric] intro!: upred_entails_exchange[OF 
-    upred_entail_eqR[OF ownE_op_minus], unfolded upred_sep_assoc_eq])
-apply (rule upred_entails_trans[OF upred_entails_eq[OF upred_sep_comm2L]])
-apply (rule upred_entails_trans[OF upred_sep_comm2R])
-apply (auto simp: dsubs_op_minus[symmetric] intro!: upred_entails_exchange[OF 
-    upred_entail_eqR[OF ownE_op_minus], unfolded upred_sep_assoc_eq] upred_entails_trans[OF _ updI]
-    upred_entails_trans[OF _ except_zeroI])
-apply (rule upred_entails_trans[OF _ upred_sep_comm2R])
-by (auto simp: upred_true_sep intro!: upred_frame)
-done
-
-lemma fresh_inv_name: "\<exists>\<iota>. \<not> (\<iota> \<in>\<^sub>f E) \<and> \<iota> \<in>\<^sub>d dnames N"
 proof -
-  from infinite_names dset_of_finite_finite have "dnames N - dset_of_finite E \<noteq> DSet {}"
-    unfolding dnames_def apply (cases E) apply auto using finite_fset infinite_super apply blast 
-    using not_no_names by simp
-  then obtain \<iota> where "\<iota> \<in>\<^sub>d dnames N - dset_of_finite E" unfolding dnames_def by (cases E) auto
-  then have "\<not> (\<iota> \<in>\<^sub>f E) \<and> \<iota> \<in>\<^sub>d dnames N" apply (cases E) by (auto simp add: dnames_def fmember.rep_eq)
-  then show ?thesis by blast
-qed
+  assume assm: "P\<turnstile>Q"
+  have "\<Turnstile>{\<E>\<^sub>1, \<E>\<^sub>2}=>P \<turnstile> \<Turnstile>{\<E>\<^sub>1, \<E>\<^sub>2}=>P" by (rule upred_entails_refl)
+  then have "((wsat \<^emph> ownE \<E>\<^sub>1) -\<^emph> (\<Rrightarrow>\<^sub>b (\<diamondop> (wsat \<^emph> ownE \<E>\<^sub>2 \<^emph> P)))) \<turnstile>
+    ((wsat \<^emph> ownE \<E>\<^sub>1) -\<^emph> (\<Rrightarrow>\<^sub>b (\<diamondop> (wsat \<^emph> ownE \<E>\<^sub>2 \<^emph> P))))" by (simp add: fancy_upd_def)
+  then have "((wsat \<^emph> ownE \<E>\<^sub>1) -\<^emph> (\<Rrightarrow>\<^sub>b (\<diamondop> (wsat \<^emph> ownE \<E>\<^sub>2 \<^emph> P)))) \<^emph> (wsat \<^emph> ownE \<E>\<^sub>1) \<turnstile>
+    \<Rrightarrow>\<^sub>b (\<diamondop> (wsat \<^emph> ownE \<E>\<^sub>2 \<^emph> P))" by (rule upred_wandE)
+  then have "((wsat \<^emph> ownE \<E>\<^sub>1) -\<^emph> (\<Rrightarrow>\<^sub>b (\<diamondop> (wsat \<^emph> ownE \<E>\<^sub>2 \<^emph> P)))) \<^emph> (wsat \<^emph> ownE \<E>\<^sub>1) \<turnstile>
+    \<Rrightarrow>\<^sub>b (\<diamondop> (wsat \<^emph> ownE \<E>\<^sub>2 \<^emph> Q))" 
+    by (rule upred_entails_trans[OF _ upd_mono[OF except_zero_mono[OF upred_sep_mono[OF 
+        upred_entails_refl]], OF assm]])
+  then have "((wsat \<^emph> ownE \<E>\<^sub>1) -\<^emph> (\<Rrightarrow>\<^sub>b (\<diamondop> (wsat \<^emph> ownE \<E>\<^sub>2 \<^emph> P)))) \<turnstile>
+    ((wsat \<^emph> ownE \<E>\<^sub>1) -\<^emph> (\<Rrightarrow>\<^sub>b (\<diamondop> (wsat \<^emph> ownE \<E>\<^sub>2 \<^emph> Q))))" by (rule upred_wandI)
+  then show ?thesis by (simp add: fancy_upd_def)
+qed  
 
-lemma inv_alloc: "(\<triangleright>P) ={E}=\<^emph> (inv N P)"
-apply (auto simp: fancy_upd_def upred_sep_assoc_eq intro!: upred_wand_holdsI upred_wandI)
-apply (subst upred_sep_comm2_eq[of wsat])
-apply (rule upred_entails_trans[OF _ upd_mono,OF _ except_zero_sepR])
-apply (auto intro!: upred_entails_trans[OF _ upd_frameL] upred_frame)
-apply (rule upred_wand_holdsE)
-apply (subst upred_sep_comm)
-apply (rule upred_entails_wand_holdsR[OF _ ownI_alloc[of "\<lambda>i. i \<in>\<^sub>d dnames N"], OF _ allI[OF fresh_inv_name, of id, simplified]])
-apply (rule upd_mono)
-apply (auto intro!: upred_existsE')
-apply (subst upred_sep_comm[of wsat])
-apply (subst upred_sep_comm2_eq)
-apply (auto intro!: upred_entails_trans[OF _ except_zeroI] upred_frame)
-unfolding inv_def
-subgoal for i
-apply (rule upred_existsI[of _ _ i])
-apply (subst upred_sep_comm)
-by (auto simp: dnames_def intro!:upred_pure_impl upred_entails_conjI upred_pureI)
-done
+lemma fupd_frame_r: "((\<Turnstile>{E1,E2}=> P) \<^emph> R) ={E1,E2}=\<^emph> (P \<^emph> R)"
+apply (rule upred_wand_holdsI)
+unfolding fancy_upd_def
+apply (auto simp: upred_sep_assoc_eq)
+apply (rule upred_entails_trans[OF upred_entails_eq[OF upred_sep_comm]])
+apply (rule upred_wandI)
+apply (rule upred_entails_trans[OF upred_sep_comm2R])
+apply (auto intro!: upred_entails_substE[OF upred_wand_apply, unfolded upred_sep_assoc_eq] 
+  upd_mono_ext except_zero_mono_ext)
+apply (rule upred_entails_trans[OF upred_entails_eq[OF upred_sep_comm]])
+by auto
+
+lemma fupd_frame_mono: "R\<^emph>P\<turnstile>Q \<Longrightarrow> R \<^emph> (\<Turnstile>{E1,E2}=> P) \<turnstile> \<Turnstile>{E1,E2}=> Q"
+apply (rule upred_entails_trans[OF upred_entails_eq[OF upred_sep_comm]])
+apply (auto intro!: upred_entails_trans[OF upred_wand_holdsE[OF fupd_frame_r]] fupd_mono)
+apply (rule upred_entails_trans[OF upred_entails_eq[OF upred_sep_comm]])
+by simp
+
+
+lemma fupd_mask_subseteq: "E2\<subseteq>\<^sub>dE1 \<Longrightarrow> \<Turnstile>{E1,E2}=>\<Turnstile>{E2,E1}=>upred_emp"
+proof -
+  assume assm: "E2 \<subseteq>\<^sub>d E1"
+  then have e1: "E1 = (E1-E2)\<cdot>E2" by (simp add: camera_comm dsubs_op_minus)
+  with assm have own_e1: "ownE E1 \<stileturn>\<turnstile> ownE (E1-E2) \<^emph> ownE E2" using ownE_op_minus
+  by (metis dsubs_op_minus upred_sep_comm)
+  show ?thesis unfolding fancy_upd_def
+  apply (rule upred_wand_holdsI)
+  apply (auto simp: upred_sep_assoc_eq intro!: upred_entails_substE[OF upred_entail_eqL[OF own_e1]]
+    upred_entails_trans[OF _ updI] upred_entails_trans[OF _ except_zeroI])
+  apply (rule upred_entails_trans[OF _ upred_sep_comm2R])
+  apply (rule upred_frame)
+  apply (auto simp: upred_sep_assoc_eq intro!: upred_sep_mono upred_wandI)
+  apply (auto intro!: upred_entails_trans[OF _ updI] upred_entails_trans[OF _ except_zeroI])
+  apply (rule upred_entails_trans[OF upred_entails_eq[OF upred_sep_comm2L]])
+  apply (rule upred_entails_trans[OF upred_sep_comm2R])
+  by (auto simp: dsubs_op_minus[OF assm,symmetric] upred_true_sep intro!: upred_entails_substE[OF 
+      upred_entail_eqR[OF ownE_op_minus[OF assm]], unfolded upred_sep_assoc_eq])
+qed
+  
+lemma persistent_vs [pers_rule]: "persistent (P ={E1,E2}=> Q)"
+  unfolding view_shift_def by pers_solver
 end
