IrisCore/WorldSatisfaction.thy
@@ -1,0 +1,261 @@
+theory WorldSatisfaction
+imports Misc
+begin
+
+subsection \<open>Invariants\<close>
+
+subsubsection \<open>World satisfaction\<close>
+text \<open> 
+  Impredicative invariants are formalized as propositions which are managed by the so called
+  World Satisfaction. It holds a map of named invariants and keeps track which of them are opened 
+  (i.e. enabled/can be used thread-locally and might not hold) and which are closed 
+  (i.e. disabled/hold for all threads).
+\<close>
+
+definition own_inv :: "inv \<Rightarrow> iprop" ("Own\<^sub>i _") where
+  "own_inv i = Own(constr_inv i)"
+
+text \<open>Allocate new invariant map\<close>
+definition ownI :: "name \<Rightarrow> iprop \<Rightarrow> iprop" where
+  "ownI \<iota> P = Own\<^sub>i (map_view_frag \<iota> DfracDiscarded (Next (pre P)),\<epsilon>,\<epsilon>)"
+
+definition inv_raw :: "namespace \<Rightarrow> iprop \<Rightarrow>  iprop" where
+  "inv_raw N P \<equiv> \<exists>\<^sub>u \<iota>. ((\<upharpoonleft>(\<iota>\<in>\<^sub>d dnames N)) \<and>\<^sub>u ownI \<iota> P)"
+
+text \<open>Allocate new enabled invariant map\<close>
+definition ownE :: "name dset \<Rightarrow> iprop" where
+  "ownE E = Own\<^sub>i (\<epsilon>,E,\<epsilon>)"
+
+text \<open>Allocate new disabled invariant map\<close>
+definition ownD :: "name dfset \<Rightarrow> iprop" where
+  "ownD D = Own\<^sub>i (\<epsilon>,\<epsilon>,D)"  
+  
+definition lift_inv_fmap :: "(name,iprop) fmap \<Rightarrow> (name,pre_iprop later) fmap" where
+  "lift_inv_fmap m = Abs_fmap (map_option (Next \<circ> pre) \<circ> (fmlookup m))"
+
+lemma lift_inf_fmap_finite: "(map_option (Next \<circ> pre) \<circ> (fmlookup m)) \<in> {m. finite (dom m)}"
+  by auto
+
+text \<open>World satisfaction, i.e. the invariant that holds all invariants\<close>
+definition wsat :: iprop where
+  "wsat \<equiv> \<exists>\<^sub>u (I::(name,iprop) fmap).
+    ((Own\<^sub>i(map_view_auth (DfracOwn 1) (lift_inv_fmap I),\<epsilon>,\<epsilon>))
+    \<^emph> (sep_map_fmdom (\<lambda>\<iota>. (\<triangleright>(the (fmlookup I \<iota>))) \<^emph> ownD (DFSet {|\<iota>|}) \<or>\<^sub>u (ownE (DSet {\<iota>}))) I)
+  )"
+
+lemma pcore_id_inv: "pcore_id_pred (constr_inv (map_view_frag \<iota> DfracDiscarded (Next (pre P)), \<epsilon>, \<epsilon>))"
+  unfolding constr_inv_def prod_pcore_id_pred
+  by (simp add: \<epsilon>_pcore_id_def) (rule pcore_id_frag[OF discarded_core_id])
+
+lemma persistent_ownI [pers_rule]: "persistent (ownI \<iota> P)"
+  unfolding ownI_def own_inv_def by (rule persistent_core_own2[OF pcore_id_inv])
+
+lemma persistent_inv_raw [pers_rule]: "persistent (inv_raw N P)"
+  unfolding inv_raw_def
+  apply (rule persistent_exists)
+  apply (rule persistent_conj)
+  apply (rule persistent_pure)
+  by (rule persistent_ownI)
+
+lemma constr_inv_valid: "\<lbrakk>valid mv; valid e; valid d\<rbrakk> \<Longrightarrow> valid (constr_inv (mv,e,d))"
+  unfolding constr_inv_def by (auto simp: prod_valid_def \<epsilon>_valid)
+
+lemma ownE_singleton_twice: "ownE (DSet {i}) \<^emph> ownE (DSet {i}) \<turnstile> \<upharpoonleft>False"
+  unfolding ownE_def own_inv_def constr_inv_def
+  apply (rule upred_entails_trans[OF upred_entail_eqR[OF own_op]])
+  apply (rule upred_entails_trans[OF own_valid])
+  apply (simp add: op_prod_def \<epsilon>_left_id op_dset_def)
+  apply transfer
+  by (simp add: prod_n_valid_def \<epsilon>_n_valid valid_raw_dset_def)
+
+lemma ownD_singleton_twice: "ownD (DFSet {|i|}) \<^emph> ownD (DFSet {|i|}) \<turnstile> \<upharpoonleft>False"
+  unfolding ownD_def own_inv_def constr_inv_def
+  apply (auto simp: op_prod_def \<epsilon>_left_id op_dfset_def
+    intro!: upred_entails_trans[OF upred_entail_eqR[OF own_op]] upred_entails_trans[OF own_valid])
+  apply transfer
+  by (simp add: prod_n_valid_def \<epsilon>_n_valid valid_raw_dfset_def)
+  
+lemma ownE_op: "(\<exists>E1' E2'. dset_raw E1 = Some E1' \<and> dset_raw E2 = Some E2' \<and> E1' \<inter> E2' = {})
+  \<Longrightarrow> ownE (E1 \<cdot> E2) \<stileturn>\<turnstile> ownE E1 \<^emph> ownE E2"
+proof -
+  assume "\<exists>E1' E2'. dset_raw E1 = Some E1' \<and> dset_raw E2 = Some E2' \<and> E1' \<inter> E2' = {}"
+  then obtain E1' E2' where assms: "dset_raw E1 = Some E1'" "dset_raw E2 = Some E2'" "E1' \<inter> E2' = {}"
+    by auto
+  then have "E1 = DSet E1'" "E2 = DSet E2'" by (metis dset_raw.elims option.discI option.inject)+
+  with assms(3) have un_op:"DSet (E1' \<union> E2') = E1 \<cdot> E2" unfolding op_dset_def by simp
+  from own_op[of "constr_inv (\<epsilon>,E1,\<epsilon>)" "constr_inv (\<epsilon>,E2,\<epsilon>)"] 
+  have "ownE (E1 \<cdot> E2) \<stileturn>\<turnstile> ownE E1 \<^emph> ownE E2"
+    by (simp add: ownE_def own_inv_def constr_inv_def op_prod_def \<epsilon>_left_id)
+  with un_op show ?thesis by simp
+qed
+
+lemma ownE_op_minus: "E1 \<subseteq>\<^sub>d E2 \<Longrightarrow> ownE (E1 \<cdot> (E2-E1)) \<stileturn>\<turnstile> ownE E1 \<^emph> ownE (E2-E1)"
+proof -
+  assume "E1 \<subseteq>\<^sub>d E2"
+  then have "\<exists>E1' E2'. dset_raw E1 = Some E1' \<and> dset_raw (E2-E1) = Some E2' \<and> E1' \<inter> E2' = {}"
+    using dsubs_dset dsubs_minus_inter by fastforce
+  from ownE_op[OF this] show ?thesis .
+qed
+  
+lemma auth_map_both_validI: 
+  "\<V>(constr_inv (map_view_auth (DfracOwn 1) m,\<epsilon>,\<epsilon>) \<cdot> constr_inv (map_view_frag k dq v,\<epsilon>,\<epsilon>)) \<turnstile>
+    (fmlookup m k =\<^sub>u Some v) \<and>\<^sub>u \<upharpoonleft>(valid dq)"
+unfolding constr_inv_def op_prod_def
+apply (simp add: \<epsilon>_left_id auth_comb_opL split: prod.splits)
+apply transfer'
+apply (simp add: prod_n_valid_def \<epsilon>_n_valid valid_raw_option_def \<epsilon>_option_def)
+using map_view_both_valid by fastforce
+
+lemma invariant_lookup: 
+  "Own\<^sub>i (map_view_auth (DfracOwn 1) (lift_inv_fmap I),\<epsilon>,\<epsilon>) \<^emph> ownI \<iota> P \<turnstile> 
+  (\<exists>\<^sub>u Q. \<upharpoonleft>(fmlookup I \<iota> = Some Q) \<^emph> \<triangleright>(Q=\<^sub>uP))"
+  unfolding ownI_def own_inv_def
+  apply (rule upred_entails_trans[OF upred_entail_eqR[OF own_op]])
+  apply (rule upred_entails_trans[OF own_valid])
+  apply (rule upred_entails_trans[OF auth_map_both_validI])
+  apply transfer'
+  apply (auto simp: lift_inv_fmap_def valid_raw_dfrac_def valid_def n_equiv_option_def 
+    n_equiv_later_def Abs_fmap_inverse[OF lift_inf_fmap_finite])
+  apply (metis dual_order.refl n_incl_def ofe_refl prod_cases3 total_n_inclI)
+  by (metis \<epsilon>_left_id ofe_refl prod_cases3) 
+
+lemma lookup_pers [pers_rule]: "persistent (\<exists>\<^sub>u Q. \<upharpoonleft>(fmlookup I \<iota> = Some Q) \<^emph> \<triangleright>(Q=\<^sub>uP))"
+  by pers_solver
+
+lemma ownI_open: "wsat \<^emph> ownI i P \<^emph> ownE (DSet {i}) \<turnstile> wsat \<^emph> (\<triangleright>P) \<^emph> ownD (DFSet {|i|})"
+unfolding wsat_def
+apply (rule pull_exists_antecedent2)
+apply (rule upred_existsE')
+apply (rule upred_entails_trans[OF upred_entails_eq[OF upred_sep_comm]])
+apply (rule upred_entails_trans[OF upred_sep_assoc])
+apply (rule upred_entails_trans[OF upred_sep_assoc'])
+apply (rule upred_entails_trans[OF upred_sep_comm3M])
+apply (rule upred_entails_trans[OF upred_sep_assoc_rev])
+apply (rule upred_entails_substE[OF  persistent_keep[OF lookup_pers invariant_lookup]])
+apply (rule upred_entails_trans[OF upred_sep_assoc])
+apply (rule pull_exists_antecedentR)
+apply (rule upred_existsE')
+apply (rule upred_entails_trans[OF upred_sep_assoc])
+apply (rule upred_entails_trans[OF upred_entails_eq[OF upred_sep_comm]])
+apply (rule upred_entails_trans[OF upred_sep_assoc])
+apply (rule upred_pure_impl)
+apply (rule upred_entails_trans[OF upred_sep_assoc])
+apply (rule upred_entails_trans[OF upred_entails_eq[OF upred_sep_comm]])
+apply (rule upred_entails_trans[OF upred_sep_assoc])+
+apply (simp add: sep_map_dom_delete)
+apply (rule upred_entails_trans[OF upred_sep_assoc])
+apply (rule upred_entails_trans[OF upred_sep_comm2R])
+apply (rule upred_disjE')
+subgoal for I Q
+  apply (rule upred_entails_trans[OF upred_sep_assoc])
+  apply (rule upred_frame)
+  apply (rule upred_entails_trans[OF upred_sep_comm4_2])
+  apply (rule upred_entails_trans[OF upred_sep_comm3M])
+  apply (rule persistent_split[OF persistent_later[OF persistent_eq]])
+  subgoal
+    apply (rule upred_entails_trans[OF upred_entail_eqR[OF upred_later_sep]])
+    apply (rule upred_later_mono)
+    apply (rule upred_entails_trans[OF upred_entails_eq[OF upred_sep_comm]])
+    apply (simp add: upred_eq_comm)
+    apply (rule upred_eqE)
+  by simp
+  apply(rule upred_existsI[of _ _ "I"])
+  apply (rule upred_entails_trans[OF upred_entails_eq[OF upred_sep_comm]])
+  apply (rule upred_entails_trans[OF upred_sep_assoc])
+  apply (rule upred_entails_trans[OF upred_entails_eq[OF upred_sep_comm]])
+  apply (rule upred_entails_trans[OF upred_sep_assoc])+
+  apply (rule upred_entails_trans[OF upred_entails_eq[OF upred_sep_comm]])
+  apply (rule upred_entails_trans[OF upred_sep_assoc])+
+  apply (rule upred_entails_trans[OF upred_entails_eq[OF upred_sep_comm]])
+  apply (rule upred_entails_trans[OF upred_sep_assoc])
+  apply (rule upred_entails_trans[OF _ upred_entails_eq[OF upred_sep_comm]])
+  apply (rule upred_frame)
+  apply (simp add: sep_map_dom_delete)
+  apply (rule upred_entails_trans[OF upred_sep_assoc])+
+  apply (rule upred_entails_trans[OF upred_sep_comm2R])
+  apply (rule upred_frame)
+  apply (rule upred_disjIR)
+  apply (rule upred_entails_trans[OF upred_sep_comm2R])
+by (rule upred_weakeningR)
+apply (rule upred_entails_trans[OF upred_entails_eq[OF upred_sep_comm2L]])
+apply (rule upred_entails_trans[OF upred_sep_assoc'])
+apply (rule upred_entails_trans[OF upred_sep_assoc_rev])
+apply (rule upred_entails_substE[OF ownE_singleton_twice])
+by simp
+
+lemma ownI_close: "wsat \<^emph> ownI i P \<^emph> (\<triangleright> P) \<^emph> ownD (DFSet {|i|}) \<turnstile> wsat \<^emph> ownE (DSet {i})"
+apply (simp add: wsat_def)
+apply (auto simp: pull_exists_eq intro!: upred_existsE')
+apply (rule upred_entails_trans[OF upred_sep_comm3M])
+apply (rule upred_entails_trans[OF upred_sep_comm2R])
+apply (rule upred_entails_trans[OF upred_entails_eq[OF upred_sep_comm2L]])
+apply (auto simp: upred_sep_assoc_eq)
+apply (rule upred_entails_trans[OF upred_sep_comm4_2])
+apply (rule upred_entails_trans[OF upred_entails_eq[OF upred_sep_comm2L]])
+apply (auto simp: upred_sep_assoc_eq)
+apply (rule upred_entails_substE[OF persistent_keep[OF lookup_pers invariant_lookup], unfolded upred_sep_assoc_eq])
+subgoal for I 
+apply (auto simp: upred_sep_assoc_eq intro!: upred_existsI[of _ _ I] pull_exists_antecedentR upred_existsE')
+apply (rule upred_entails_trans[OF upred_sep_comm2R])
+apply (auto simp: sep_map_dom_delete upred_sep_assoc_eq intro!: upred_pure_impl)
+apply (rule upred_entails_trans[OF upred_entails_eq[OF upred_sep_comm]])
+apply (simp add: upred_sep_assoc_eq)
+apply (rule upred_entails_trans[OF upred_sep_comm4_2])
+apply (rule upred_entails_trans[OF upred_sep_comm3M])
+apply (rule upred_entails_trans[OF upred_sep_comm2R])
+apply (auto simp: upred_sep_assoc_eq intro!: upred_disjE')
+subgoal for Q  
+  apply (rule upred_entails_trans[OF upred_sep_comm6_2R])
+  by (auto intro!: upred_entails_substE[OF ownD_singleton_twice, unfolded upred_sep_assoc_eq])
+apply (auto simp: upred_sep_assoc_eq intro!: upred_frame)
+apply (rule upred_entails_trans[OF upred_entails_eq[OF upred_sep_comm2L]])
+apply (rule upred_entails_trans[OF upred_sep_comm2R])
+apply (auto simp: upred_sep_assoc_eq intro!: upred_frame)
+apply (rule upred_entails_trans[OF upred_entails_eq[OF upred_sep_comm2L]])
+apply (simp add: upred_sep_assoc_eq)
+apply (rule upred_entails_trans[OF upred_sep_comm4_2])
+apply (rule upred_entails_trans[OF upred_sep_comm3M])
+apply (rule upred_entails_trans[OF upred_sep_comm2R])
+apply (rule upred_entails_trans[OF _ upred_entails_eq[OF upred_sep_comm]])
+apply (auto simp: upred_sep_assoc_eq intro!: upred_frame upred_disjIL)
+apply (rule upred_entails_trans[OF upred_entails_eq[OF upred_sep_comm2L]])
+by (auto intro!: upred_entails_trans[OF upred_weakeningR2] 
+  upred_entails_trans[OF upred_entail_eqR[OF upred_later_sep]] upred_later_mono upred_eqE)
+done
+
+lemma ownI_alloc: "(\<forall>E::name dfset. \<exists>i. \<not>i\<in>\<^sub>fE \<and> \<phi> i) \<Longrightarrow> 
+  (wsat \<^emph> \<triangleright> P) ==\<^emph> (\<exists>\<^sub>u i. \<upharpoonleft>(\<phi> i) \<^emph> wsat \<^emph> ownI i P)"
+apply (auto simp: wsat_def pull_exists_eq intro!: upred_wand_holdsI upred_existsE')
+apply (rule add_holds[OF own_unit,unfolded bupd_emp[OF upred_own_nothing_emp_eq]])
+apply (rule upred_entails_substE[OF upred_wand_holdsE[OF own_updateP]])
+sorry (* Axiomatized as this requires too much low level ghost state reasoning for which I'd need to add
+    way more lemmata and things. *)
+
+lemma ownI_alloc_open: "(\<forall>E::name dfset. \<exists>i. \<not>i\<in>\<^sub>fE \<and> \<phi> i) \<Longrightarrow> 
+  wsat ==\<^emph> (\<exists>\<^sub>u i. \<upharpoonleft>(\<phi> i) \<^emph> (ownE (DSet {i}) -\<^emph> wsat) \<^emph> ownI i P \<^emph> ownD (DFSet {|i|}))"
+apply (auto simp: wsat_def pull_exists_eq intro!: upred_wand_holdsI upred_existsE')
+sorry (* Axiomatized as this requires too much low level ghost state reasoning for which I'd need to add
+    way more lemmata and things. *)
+
+lemma wsat_alloc: "\<Rrightarrow>\<^sub>b (\<exists>\<^sub>u _::inv. wsat \<^emph> ownE (DSet UNIV))"
+apply (auto simp: upred_holds_entails)
+apply (rule add_own[of "constr_inv (map_view_auth (DfracOwn 1) fmempty,\<epsilon>,\<epsilon>)", 
+  OF constr_inv_valid[OF map_view_auth_valid \<epsilon>_valid \<epsilon>_valid]])
+apply (rule add_own[of "constr_inv (\<epsilon>,DSet UNIV,\<epsilon>)", 
+  OF constr_inv_valid[OF \<epsilon>_valid _ \<epsilon>_valid]])
+apply (simp add: valid_raw_dset_def valid_def)
+apply (rule add_own[of "constr_inv (\<epsilon>,\<epsilon>,DFSet {||})", 
+  OF constr_inv_valid[OF \<epsilon>_valid \<epsilon>_valid _], unfolded \<epsilon>_dfset_def[symmetric], OF \<epsilon>_valid])
+apply (auto simp: wsat_def pull_exists_eq own_inv_def ownE_def ownD_def 
+  intro!: upred_entails_trans[OF _ updI])
+apply (rule upred_existsI)
+apply (rule upred_existsI[of _ _ fmempty])
+apply (rule upred_entails_trans[OF upred_sep_comm2R])
+apply (auto intro!: upred_frame)
+apply (auto simp: lift_inv_fmap_def fmempty.rep_eq fmempty_def[symmetric] sep_fold_fset_def 
+  comp_fun_commute.ffold_empty[OF sep_P_comp_fun_commute]  intro!: upred_frame)
+apply (rule upred_entails_trans[OF upred_entails_eq[OF upred_sep_comm2L]])
+apply (rule upred_entails_trans[OF upred_sep_comm2R])
+by (auto simp: upred_weakeningL intro!: upred_frame)
+
+end
